PathDependent/LambdaP/Cont.lean
@@ -1,0 +1,33 @@
+import PathDependent.FinFun.Basic
+import PathDependent.LambdaP.Syntax
+
+namespace LambdaP.Cont
+
+  open LambdaP.Syntax
+  open FinFun
+
+  -- We model continuations as stacks (i.e. lists) of frames
+
+  inductive Path.Frame: Type
+  | fst  : Frame
+  | sel  : Name -> Frame
+
+  inductive Tm.Frame: Nat -> Type
+  | path  : Frame n
+  | let   : Tm (n + 1) -> Frame n
+  | app_l : Path n -> Frame n
+  | app_r : Fin n -> Frame n
+
+  def Path.Cont := List Path.Frame
+  def Tm.Cont (n: Nat) := List (Tm.Frame n)
+
+  def Tm.Frame.rename (F: Tm.Frame n) (f: FinFun n m): Tm.Frame m := match F with
+  | Tm.Frame.path => Tm.Frame.path
+  | Tm.Frame.let t => Tm.Frame.let (t.rename f.ext)
+  | app_l p => app_l (p.rename f)
+  | app_r x => app_r (f x)
+
+  def Tm.Frame.weaken (F : Tm.Frame n): Tm.Frame (n + 1) := F.rename FinFun.weaken
+  def Tm.Cont.weaken: Tm.Cont n -> Tm.Cont (n + 1) := List.map Tm.Frame.weaken
+
+end LambdaP.Cont
