PathDependent/LambdaP/Reduction.lean
@@ -1,0 +1,56 @@
+import PathDependent.LambdaP.Syntax
+import PathDependent.LambdaP.Cont
+import PathDependent.LambdaP.Store
+
+namespace LambdaP.Reduction
+
+  open LambdaP.Syntax
+  open LambdaP.Cont
+  open LambdaP.Store
+
+  structure State (n: Nat) where
+    σ    : Store n
+    cont_tm : Tm.Cont n
+    cont_path : Path.Cont
+    term : Tm n
+
+  inductive State.Step : State n -> State m -> Prop
+  | app_push_l {σ : Store n} :
+        Step ⟨σ, k, [], Tm.app p q⟩ ⟨σ, Tm.Frame.app_l q :: k, [], Tm.path p⟩
+
+  | app_push_r {σ : Store n} :
+        Step ⟨σ, Tm.Frame.app_l q :: k, [], Tm.path (Path.var x) ⟩ ⟨σ, Tm.Frame.app_r x :: k, [], Tm.path q⟩
+
+  | app {σ : Store n} :
+        σ.Binds x (Tm.abs T t) ->
+        Step ⟨σ, Tm.Frame.app_r x :: k, [], Tm.path (Path.var y)⟩ ⟨σ, k, [], t.open y⟩
+
+  | let_push {σ : Store n} :
+        Step ⟨σ, k, [], Tm.let s t⟩ ⟨σ, Tm.Frame.let t :: k, [], s⟩
+
+  | rename {σ : Store n} :
+        Step ⟨σ, Tm.Frame.let t :: k, [], Tm.path (Path.var x)⟩ ⟨σ, k, [], t.open x ⟩
+
+  | lift {σ : Store n} :
+        (vv : Tm.IsValue v) ->
+        Step ⟨σ, Tm.Frame.let t :: k, [], v⟩ ⟨σ.val v vv, Tm.Cont.weaken k, [], t ⟩
+
+  | ascribe {σ : Store n} :
+        Step ⟨σ, k, [], Tm.typed t T⟩ ⟨σ, k, [], t⟩
+
+  | fst_push {σ : Store n} :
+        Step ⟨σ, k, p, Tm.path (Path.fst q)⟩ ⟨σ, k, Path.Frame.fst :: p, q⟩
+
+  | fst {σ : Store n} :
+        σ.Binds x (Tm.pair y α δ) ->
+        Step ⟨σ, k, Path.Frame.fst :: p, Tm.path (Path.var x)⟩ ⟨σ, k, p, Tm.path (Path.var y) ⟩
+
+  | sel_push {σ : Store n} :
+        Step ⟨σ, k, p, Tm.path (Path.sel q a)⟩ ⟨σ, k, Path.Frame.sel a :: p, q⟩
+
+  | sel {σ : Store n} :
+        σ.Binds x (Tm.pair y a (Def.val z)) ->
+        Step ⟨σ, k, Path.Frame.sel a :: p, Tm.path (Path.var x)⟩ ⟨σ, k, p, Tm.path (Path.var z) ⟩
+
+
+end LambdaP.Reduction
