PathDependent/LambdaP/Store.lean
@@ -1,0 +1,17 @@
+import PathDependent.LambdaP.Syntax
+
+namespace LambdaP.Store
+  open LambdaP.Syntax
+
+  inductive Store: Nat -> Type
+  | empty : Store n
+  | val : Store n -> (t: Tm n) -> t.IsValue -> Store (n + 1)
+
+  inductive Store.Binds: Store n -> Fin n -> Tm n -> Prop
+  | here:  Binds (val σ v vv) 0 v.weaken
+  | there: Binds σ x v -> Binds (σ.val u uv) (Fin.succ x) v.weaken
+
+  lemma Store.Binds.IsValue: Store.Binds σ x v -> v.IsValue := by
+    sorry
+
+end LambdaP.Store
